Matroid/Order/Weak.lean
@@ -1,0 +1,73 @@
+import Matroid.Minor.Rank
+import Matroid.Flat.Hyperplane
+
+universe u
+
+open Set
+namespace Matroid
+
+variable {α : Type*} {M N M₁ M₂ : Matroid α} {X Y F : Set α}
+
+section Weak
+
+variable {I B D : Set α}
+
+@[mk_iff]
+structure WeakLE (N M : Matroid α) : Prop where
+  forall_indep_of_indep : ∀ I, N.Indep I → M.Indep I
+  ground_eq : N.E = M.E
+
+infixl:50 " ≤w " => Matroid.WeakLE
+
+@[aesop unsafe 10% (rule_sets := [Matroid])]
+lemma WeakLE.subset_ground_of_subset_ground_left (h : N ≤w M) (hX : X ⊆ N.E := by aesop_mat) :
+    X ⊆ M.E :=
+  hX.trans h.ground_eq.subset
+
+@[aesop unsafe 10% (rule_sets := [Matroid])]
+lemma WeakLE.subset_ground_of_subset_ground_right (h : N ≤w M) (hX : X ⊆ M.E := by aesop_mat) :
+    X ⊆ N.E :=
+  hX.trans h.ground_eq.symm.subset
+
+lemma WeakLE.indep_of_indep (h : N ≤w M) (hI : N.Indep I) : M.Indep I :=
+  h.forall_indep_of_indep _ hI
+
+lemma WeakLE.dep_of_dep (h : N ≤w M) (hD : M.Dep D) : N.Dep D := by
+  have hIN := h.subset_ground_of_subset_ground_right hD.subset_ground
+  contrapose! hD
+  rw [not_dep_iff] at hD ⊢
+  exact h.indep_of_indep hD
+
+lemma weakLE_iff_forall_dep_of_dep : N ≤w M ↔ N.E = M.E ∧ ∀ D, M.Dep D → N.Dep D := by
+  refine ⟨fun h ↦ ⟨h.ground_eq, fun _ ↦ h.dep_of_dep⟩, fun h ↦ ⟨fun D hD ↦ ?_, h.1⟩⟩
+  have hDN : D ⊆ N.E := hD.subset_ground
+  have hDM : D ⊆ M.E := hDN.trans_eq h.1
+  contrapose! hD
+  rw [not_indep_iff] at hD ⊢
+  exact h.2 _ hD
+
+lemma WeakLE.refl (M : Matroid α) : M ≤w M where
+  forall_indep_of_indep := by simp
+  ground_eq := rfl
+
+lemma WeakLE.antisymm (h : N ≤w M) (h' : M ≤w N) : N = M :=
+  ext_indep h.ground_eq fun _ _ ↦ ⟨h.indep_of_indep, h'.indep_of_indep⟩
+
+lemma WeakLE.trans {M₁ M₂ M₃ : Matroid α} (h : M₁ ≤w M₂) (h' : M₂ ≤w M₃) : M₁ ≤w M₃ where
+  forall_indep_of_indep _ := h'.indep_of_indep ∘ h.indep_of_indep
+  ground_eq := h.ground_eq.trans h'.ground_eq
+
+lemma WeakLE.delete (h : N ≤w M) (D : Set α) : N ＼ D ≤w M ＼ D := by
+  suffices ∀ (I : Set α), N.Indep I → Disjoint I D → M.Indep I by
+    simpa (config := { contextual := true }) [weakLE_iff, h.ground_eq]
+  exact fun I hI _ ↦ h.indep_of_indep hI
+
+lemma contract_weakLE_delete (M : Matroid α) (X : Set α) : M ／ X ≤w M ＼ X := by
+  obtain ⟨I, hI⟩ := M.exists_basis' X
+  rw [hI.contract_eq_contract_delete]
+  simp only [weakLE_iff, delete_indep_iff, hI.indep.contract_indep_iff, and_imp, delete_ground,
+    contract_ground, diff_diff, union_diff_self, union_eq_self_of_subset_left hI.subset, and_true]
+  refine fun J hJI hi hJ'  ↦ ⟨hi.subset subset_union_left, ?_⟩
+  simpa only [diff_union_self, disjoint_union_right, and_iff_left hJI] using hJ'.union_right hJI
+
+end Weak
